ast: Fill in most C# AST to Entity translations

src/AST/Translator.Expressions.dfy
@@ -556,55 +556,74 @@ module Bootstrap.AST.Translator {
   }
   */
 
-  function method TranslateName(str: System.String): N.Name {
+  function method TranslateName(str: System.String): TranslationResult<N.Name> {
     var name := TypeConv.AsString(str);
     var parts := Seq.Split('.', name);
-    assume forall s | s in parts :: s != "";
+    :- Need(forall s | s in parts :: s != "", Invalid("Empty component in name"));
     assert forall s | s in parts :: '.' !in s;
     assert forall s | s in parts :: s != "" && '.' !in s;
     var atoms : seq<N.Atom> := parts;
-    Seq.FoldL((n: N.Name, a: N.Atom) => N.Name(n, a), N.Anonymous, atoms)
+    Success(Seq.FoldL((n: N.Name, a: N.Atom) => N.Name(n, a), N.Anonymous, atoms))
   }
 
-  function method TranslateImports(md: C.ModuleDecl): (imps: TranslationResult<seq<E.Import>>)
-    reads *
-  {
-    Failure(Invalid("NYI"))
+  function method TranslateAttributeName(s: string): E.AttributeName {
+    match s {
+      case "axiom" => E.AttributeName.Axiom
+      case "extern" => E.AttributeName.Extern
+      case _ => E.AttributeName.UserAttribute(s)
+    }
   }
 
-  function method TranslateExportSet(md: C.ModuleDecl): (exps: TranslationResult<E.ExportSet>)
+  function method TranslateAttributes(attrs: C.Attributes): TranslationResult<seq<E.Attribute>>
     reads *
   {
-    Failure(Invalid("NYI"))
+    var name := TypeConv.AsString(attrs.Name);
+    var args :- Seq.MapResult(ListUtils.ToSeq(attrs.Args), TranslateExpression);
+    // TODO: Attributes needs to be nullable
+    //var rest :- if attrs.Prev == null then Success([]) else TranslateAttributes(attrs.Prev);
+    var rest := [];
+    Success([E.Attribute.Attribute(TranslateAttributeName(name), args)] + rest)
   }
 
-  function method TranslateField(f: C.Field): (d: TranslationResult<E.Definition>)
+  function method TranslateField(f: C.Field): (d: TranslationResult<E.Entity>)
     reads *
   {
+    var name :- TranslateName(f.FullDafnyName);
+    var attrs :- TranslateAttributes(f.Attributes);
     var kind := if f.IsMutable then E.Var else E.Const;
-    var name := f.FullDafnyName;
-    Failure(Invalid("NYI"))
+    var ei := E.EntityInfo(name, attrs := attrs, members := []);
+    if f is C.ConstantField then
+      var init :- TranslateExpression((f as C.ConstantField).Rhs);
+      Success(E.Definition(ei, E.Definition.Field(E.Field.Field(kind, Some(init)))))
+    else
+      Success(E.Definition(ei, E.Definition.Field(E.Field.Field(kind, None))))
   }
 
-  function method TranslateMethod(m: C.Method): (d: TranslationResult<E.Definition>)
+  function method TranslateMethod(m: C.Method): (d: TranslationResult<E.Entity>)
     reads *
   {
+    var name :- TranslateName(m.FullDafnyName);
+    var attrs :- TranslateAttributes(m.Attributes);
     var body :- TranslateStatement(m.Body);
     var def := if m is C.Constructor then
                  E.Constructor(body)
                else
                  E.Method(body);
-    Success(E.Callable(def))
+    var ei := E.EntityInfo(name, attrs := attrs, members := []);
+    Success(E.Definition(ei, E.Callable(def)))
   }
 
-  function method TranslateFunction(f: C.Function): (d: TranslationResult<E.Definition>)
+  function method TranslateFunction(f: C.Function): (d: TranslationResult<E.Entity>)
     reads *
   {
+    var name :- TranslateName(f.FullDafnyName);
+    var attrs :- TranslateAttributes(f.Attributes);
     var body :- TranslateExpression(f.Body);
-    Success(E.Callable(E.Function(body)))
+    var ei := E.EntityInfo(name, attrs := attrs, members := []);
+    Success(E.Definition(ei, E.Callable(E.Function(body))))
   }
 
-  function method TranslateMemberDecl(md: C.MemberDecl): (d: TranslationResult<E.Definition>)
+  function method TranslateMemberDecl(md: C.MemberDecl): (d: TranslationResult<E.Entity>)
     reads *
   {
     if md is C.Field then
@@ -617,63 +636,85 @@ module Bootstrap.AST.Translator {
       Failure(Invalid("Unsupported member declaration type"))
   }
 
-  function method TranslateValueTypeDecl(vt: C.ValuetypeDecl): (e: TranslationResult<seq<E.Entity>>)
+  function method TranslateTypeSynonymDecl(ts: C.TypeSynonymDecl): (e: TranslationResult<E.Type>)
     reads *
   {
-    Failure(Invalid("NYI"))
+    var ty :- TranslateType(ts.Rhs);
+    Success(E.Type.TypeAlias(E.TypeAlias.TypeAlias(ty)))
   }
 
-  function method TranslateTypeSynonymDecl(ts: C.TypeSynonymDecl): (e: TranslationResult<seq<E.Entity>>)
+  function method TranslateOpaqueTypeDecl(ot: C.OpaqueTypeDecl): (e: TranslationResult<E.Type>)
     reads *
   {
-    Failure(Invalid("NYI"))
+    Success(E.Type.AbstractType(E.AbstractType.AbstractType()))
   }
 
-  function method TranslateOpaqueTypeDecl(ot: C.OpaqueTypeDecl): (e: TranslationResult<seq<E.Entity>>)
+  function method TranslateNewtypeDecl(nt: C.NewtypeDecl): (e: TranslationResult<E.Type>)
     reads *
   {
-    Failure(Invalid("NYI"))
+    Success(E.Type.NewType(E.NewType.NewType()))
   }
 
-  function method TranslateNewtypeDecl(nt: C.NewtypeDecl): (e: TranslationResult<seq<E.Entity>>)
+  function method TranslateDatatypeDecl(dt: C.DatatypeDecl): (e: TranslationResult<E.Type>)
     reads *
   {
-    Failure(Invalid("NYI"))
+    Success(E.Type.DataType(E.DataType.DataType()))
   }
 
-  function method TranslateDatatypeDecl(dt: C.DatatypeDecl): (e: TranslationResult<seq<E.Entity>>)
+  function method TranslateTraitDecl(t: C.TraitDecl): (e: TranslationResult<E.Type>)
     reads *
   {
-    Failure(Invalid("NYI"))
+    var parentTraits :- Seq.MapResult(ListUtils.ToSeq(t.ParentTraits), (t: C.Type) reads * =>
+      TranslateName(t.AsTraitType.FullDafnyName));
+    Success(E.Type.TraitType(E.TraitType.TraitType(parentTraits)))
   }
 
-  function method TranslateTraitDecl(t: C.TraitDecl): (e: TranslationResult<seq<E.Entity>>)
+  function method TranslateClassDecl(c: C.ClassDecl): (e: TranslationResult<E.Type>)
     reads *
   {
-    Failure(Invalid("NYI"))
+    var parentTraits :- Seq.MapResult(ListUtils.ToSeq(c.ParentTraits), (t: C.Type) reads * =>
+      TranslateName(t.AsTraitType.FullDafnyName));
+    Success(E.Type.ClassType(E.ClassType.ClassType(parentTraits)))
   }
 
-  function method TranslateClassDecl(c: C.ClassDecl): (e: TranslationResult<seq<E.Entity>>)
+  function method TranslateEntityInfo(tl: C.TopLevelDecl): (e: TranslationResult<E.EntityInfo>)
     reads *
   {
-    Failure(Invalid("NYI"))
+    var name :- TranslateName(tl.FullDafnyName);
+    var attrs :- TranslateAttributes(tl.Attributes);
+    Success(E.EntityInfo(name, attrs := attrs, members := []))
+  }
+
+  function method TranslateEntityInfoMembers(tl: C.TopLevelDeclWithMembers): (e: TranslationResult<(seq<E.Entity>, E.EntityInfo)>)
+    reads *
+  {
+    var name :- TranslateName(tl.FullDafnyName);
+    var attrs :- TranslateAttributes(tl.Attributes);
+    var memberDecls := ListUtils.ToSeq(tl.Members);
+    var members :- Seq.MapResult(memberDecls, d reads * => TranslateMemberDecl(d));
+    var memberNames := Seq.Map((m: E.Entity) => m.ei.name, members);
+    :- Need(forall nm <- memberNames :: nm.ChildOf(name), Invalid("Malformed name"));
+    Success((members, E.EntityInfo(name, attrs := attrs, members := memberNames)))
   }
 
   function method TranslateTopLevelDeclWithMembers(tl: C.TopLevelDeclWithMembers): (e: TranslationResult<seq<E.Entity>>)
     reads *
   {
-    if tl is C.OpaqueTypeDecl then
-      TranslateOpaqueTypeDecl(tl)
-    else if tl is C.NewtypeDecl then
-      TranslateNewtypeDecl(tl)
-    else if tl is C.DatatypeDecl then
-      TranslateDatatypeDecl(tl)
-    else if tl is C.TraitDecl then
-      TranslateTraitDecl(tl)
-    else if tl is C.ClassDecl then
-      TranslateClassDecl(tl)
-    else
-      Failure(Invalid("Unsupported top level declaration type"))
+    var (members, ei) :- TranslateEntityInfoMembers(tl);
+    var top :- if tl is C.OpaqueTypeDecl then
+                 TranslateOpaqueTypeDecl(tl)
+               else if tl is C.NewtypeDecl then
+                 TranslateNewtypeDecl(tl)
+               else if tl is C.DatatypeDecl then
+                 TranslateDatatypeDecl(tl)
+               else if tl is C.TraitDecl then
+                 TranslateTraitDecl(tl)
+               else if tl is C.ClassDecl then
+                 TranslateClassDecl(tl)
+               else
+                 Failure(Invalid("Unsupported top level declaration type"));
+    var topEntity := E.Entity.Type(ei, top);
+    Success([topEntity] + members)
   }
 
   function method TranslateTopLevelDecl(tl: C.TopLevelDecl): (exps: TranslationResult<seq<E.Entity>>)
@@ -682,8 +723,6 @@ module Bootstrap.AST.Translator {
   {
     if tl is C.TopLevelDeclWithMembers then
       TranslateTopLevelDeclWithMembers(tl)
-    else if tl is C.ValuetypeDecl then
-      TranslateValueTypeDecl(tl)
     else if tl is C.ModuleDecl then
       var md := tl as C.ModuleDecl;
       assume ASTHeight(md.Signature) < ASTHeight(tl);
@@ -696,8 +735,8 @@ module Bootstrap.AST.Translator {
     reads *
     decreases ASTHeight(sig), 1
   {
-    var name := TranslateName(sig.ModuleDef.FullName);
-    var attrs := sig.ModuleDef.Attributes;
+    var name :- TranslateName(sig.ModuleDef.FullDafnyName);
+    var attrs :- TranslateAttributes(sig.ModuleDef.Attributes);
     var includes := ListUtils.ToSeq(sig.ModuleDef.Includes);
     var exports := sig.ExportSets;
     var topLevels := DictUtils.DictionaryToSeq(sig.TopLevels);
@@ -706,7 +745,9 @@ module Bootstrap.AST.Translator {
         assume ASTHeight(tl.1) < ASTHeight(sig);
         TranslateTopLevelDecl(tl.1));
     var topDecls' := Seq.Flatten(topDecls);
-    var ei := E.EntityInfo.Mk(name); // TODO
+    var topNames := Seq.Map((d: E.Entity) => d.ei.name, topDecls');
+    :- Need(forall nm <- topNames :: nm.ChildOf(name), Invalid("Malformed name"));
+    var ei := E.EntityInfo(name, attrs := attrs, members := topNames);
     var mod := E.Entity.Module(ei, E.Module.Module());
     Success([mod] + topDecls')
   }
@@ -718,8 +759,8 @@ module Bootstrap.AST.Translator {
     var entities :- Seq.MapResult(moduleSigs,
       (sig: (C.ModuleDefinition, C.ModuleSignature)) reads * => TranslateModule(sig.1));
     var regMap := Seq.FoldL((m:map<N.Name, E.Entity>, e: E.Entity) => m + map[e.ei.name := e], map[], Seq.Flatten(entities));
-    var mainMethodName := TranslateName(p.MainMethod.FullName);
-    var defaultModuleName := TranslateName(p.DefaultModule.FullName);
+    var mainMethodName :- TranslateName(p.MainMethod.FullDafnyName);
+    var defaultModuleName :- TranslateName(p.DefaultModule.FullDafnyName);
     var reg := E.Registry_.Registry(regMap);
     :- Need(reg.Validate().Pass?, Invalid("Failed to validate registry"));
     var prog := E.Program(reg, defaultModule := defaultModuleName, mainMethod := Some(mainMethodName));
